theories/Core/Syntactic/CtxSub.v
@@ -49,7 +49,7 @@ Module ctxsub_judg.
     2-3: inversion_clear HΓΔ; econstructor; mautosolve 4.
 
     - (* ctxsub_exp_eq_helper variable case *)
-      inversion_clear HΓΔ as [|Δ0 ? C'].
+      inversion_clear HΓΔ as [|Δ0 ? ? C'].
       assert (exists D, {{ #x : D ∈ Δ0 }} /\ {{ Δ0 ⊢ D ⊆ B }}) as [D [i0 ?]] by mauto.
       destruct_conjs.
       assert {{ ⊢ Δ0, C' }} by mauto.
